Update sorting examples to be consistent with paper.

theories/examples/loop_sort.v
@@ -1,45 +1,104 @@
 From stdpp Require Import sorting.
-From actris.channel Require Import proto_channel.
+From actris.channel Require Import proto_channel proofmode.
 From iris.heap_lang Require Import proofmode notation.
 From actris.examples Require Import sort.
 
-Definition loop_sort_service : val :=
-  rec: "go" "c" :=
-    if: recv "c" then sort_service "c";; "go" "c"
+Definition sort_service_br : val :=
+  rec: "go" "cmp" "c" :=
+    if: ~recv "c" then #() else
+    sort_service "cmp" "c";;
+    "go" "cmp" "c".
+
+Definition sort_service_del : val :=
+  rec: "go" "cmp" "c" :=
+    if: ~recv "c" then #() else
+    send "c" (start_chan (λ: "c", sort_service "cmp" "c"));;
+    "go" "cmp" "c".
+
+Definition sort_service_br_del : val :=
+  rec: "go" "cmp" "c" :=
+    if: recv "c" then
+      sort_service "cmp" "c";;
+      "go" "cmp" "c"
     else if: recv "c" then
-      let: "d" := start_chan "go" in
-      send "c" "d";;
-      "go" "c"
+      send "c" (start_chan (λ: "c", "go" "cmp" "c"));;
+      "go" "cmp" "c"
     else #().
 
-Section loop_sort.
+Section sort_service_br_del.
   Context `{!heapG Σ, !proto_chanG Σ} (N : namespace).
+  Context {A} (I : A → val → iProp Σ) (R : A → A → Prop) `{!RelDecision R, !Total R}.
 
-  Definition loop_sort_protocol_aux (rec : iProto Σ) : iProto Σ :=
-    ((sort_protocol <++> rec) <+> ((<?> c, MSG c {{ c ↣ rec @ N }}; rec) <+> END))%proto.
-
-  Instance loop_sort_protocol_aux_contractive : Contractive loop_sort_protocol_aux.
+  Definition sort_protocol_br_aux (rec : iProto Σ) : iProto Σ :=
+    ((sort_protocol I R <++> rec) <+> END)%proto.
+  Instance sort_protocol_br_aux_contractive : Contractive sort_protocol_br_aux.
   Proof. solve_proto_contractive. Qed.
-  Definition loop_sort_protocol : iProto Σ := fixpoint loop_sort_protocol_aux.
-  Global Instance loop_sort_protocol_unfold :
-    ProtoUnfold loop_sort_protocol (loop_sort_protocol_aux loop_sort_protocol).
-  Proof. apply proto_unfold_eq, (fixpoint_unfold loop_sort_protocol_aux). Qed.
+  Definition sort_protocol_br : iProto Σ := fixpoint sort_protocol_br_aux.
+  Global Instance sort_protocol_br_unfold :
+    ProtoUnfold sort_protocol_br (sort_protocol_br_aux sort_protocol_br).
+  Proof. apply proto_unfold_eq, (fixpoint_unfold sort_protocol_br_aux). Qed.
 
-  Lemma loop_sort_service_spec c :
-    {{{ c ↣ iProto_dual loop_sort_protocol @ N }}}
-      loop_sort_service c
+  Lemma sort_service_br_spec cmp c :
+    cmp_spec I R cmp -∗
+    {{{ c ↣ iProto_dual sort_protocol_br @ N }}}
+      sort_service_br cmp c
     {{{ RET #(); c ↣ END @ N }}}.
   Proof.
-    iIntros (Ψ) "Hc HΨ". iLöb as "IH" forall (c Ψ).
-    wp_rec. wp_apply (branch_spec with "Hc"); iIntros ([]) "/= [Hc _]"; wp_if.
-    { wp_apply (sort_service_spec with "Hc"); iIntros "Hc".
+    iIntros "#Hcmp !>" (Ψ) "Hc HΨ". iLöb as "IH" forall (c Ψ).
+    wp_rec. wp_branch; wp_pures.
+    { wp_apply (sort_service_spec with "Hcmp Hc"); iIntros "Hc".
       by wp_apply ("IH" with "Hc"). }
-    wp_apply (branch_spec with "Hc"); iIntros ([]) "/= [Hc _]"; wp_if.
-    - wp_apply (start_chan_proto_spec N loop_sort_protocol); iIntros (d) "Hd".
-      { wp_apply ("IH" with "Hd"); auto. }
-      wp_apply (send_proto_spec with "Hc"); simpl.
-      iExists d; iSplit; first done. iIntros "{$Hd} !> Hc".
-      by wp_apply ("IH" with "Hc").
-    - by iApply "HΨ".
+    by iApply "HΨ".
   Qed.
-End loop_sort.
+
+  Definition sort_protocol_del_aux (rec : iProto Σ) : iProto Σ :=
+    ((<?> c, MSG c {{ c ↣ sort_protocol I R @ N }}; rec) <+> END)%proto.
+  Instance sort_protocol_del_aux_contractive : Contractive sort_protocol_del_aux.
+  Proof. solve_proto_contractive. Qed.
+  Definition sort_protocol_del : iProto Σ := fixpoint sort_protocol_del_aux.
+  Global Instance sort_protocol_del_unfold :
+    ProtoUnfold sort_protocol_del (sort_protocol_del_aux sort_protocol_del).
+  Proof. apply proto_unfold_eq, (fixpoint_unfold sort_protocol_del_aux). Qed.
+
+  Lemma sort_protocol_del_spec cmp c :
+    cmp_spec I R cmp -∗
+    {{{ c ↣ iProto_dual sort_protocol_del @ N }}}
+      sort_service_del cmp c
+    {{{ RET #(); c ↣ END @ N }}}.
+  Proof.
+    iIntros "#Hcmp !>" (Ψ) "Hc HΨ". iLöb as "IH" forall (Ψ).
+    wp_rec. wp_branch; wp_pures.
+    { wp_apply (start_chan_proto_spec _ (sort_protocol I R <++> END)%proto);
+        iIntros (c') "Hc'".
+      { wp_pures. wp_apply (sort_service_spec with "Hcmp Hc'"); auto. }
+      wp_send with "[$Hc']". by wp_apply ("IH" with "Hc"). }
+    by iApply "HΨ".
+  Qed.
+
+  Definition sort_protocol_br_del_aux (rec : iProto Σ) : iProto Σ :=
+    ((sort_protocol I R <++> rec) <+> ((<?> c, MSG c {{ c ↣ rec @ N }}; rec) <+> END))%proto.
+  Instance sort_protocol_br_del_aux_contractive : Contractive sort_protocol_br_del_aux.
+  Proof. solve_proto_contractive. Qed.
+  Definition sort_protocol_br_del : iProto Σ := fixpoint sort_protocol_br_del_aux.
+  Global Instance sort_protocol_br_del_unfold :
+    ProtoUnfold sort_protocol_br_del (sort_protocol_br_del_aux sort_protocol_br_del).
+  Proof. apply proto_unfold_eq, (fixpoint_unfold sort_protocol_br_del_aux). Qed.
+
+  Lemma sort_service_br_del_spec cmp c :
+    cmp_spec I R cmp -∗
+    {{{ c ↣ iProto_dual sort_protocol_br_del @ N }}}
+      sort_service_br_del cmp c
+    {{{ RET #(); c ↣ END @ N }}}.
+  Proof.
+    iIntros "#Hcmp !>" (Ψ) "Hc HΨ". iLöb as "IH" forall (c Ψ).
+    wp_rec. wp_branch; wp_pures.
+    { wp_apply (sort_service_spec with "Hcmp Hc"); iIntros "Hc".
+      by wp_apply ("IH" with "Hc"). }
+    wp_branch; wp_pures.
+    { wp_apply (start_chan_proto_spec N sort_protocol_br_del); iIntros (c') "Hc'".
+      { wp_apply ("IH" with "Hc'"); auto. }
+      wp_send with "[$Hc']".
+      by wp_apply ("IH" with "Hc"). }
+    by iApply "HΨ".
+  Qed.
+End sort_service_br_del.
